data model, theory

app/models/Folder.scala
@@ -1,5 +1,10 @@
 package models
 
-class Folder {
+import scala.slick.driver.H2Driver.simple._
+import Database.{threadLocalSession => session}
 
+case class Folder(id: Long, name: String, )
+
+object Folders extends Table[Folder]("folders") {
+  
 }
